src/LeanEVM/Eval.lean
@@ -1,0 +1,71 @@
+import LeanEVM.State
+import LeanEVM.Util
+import LeanEVM.Instructions.Arithmetic
+import LeanEVM.Instructions.ControlFlow
+import LeanEVM.Instructions.Stack
+
+open Bytecode
+open Exception
+open Outcome
+
+-- ==================================================================
+-- Eval(uate)
+-- ==================================================================
+
+-- Execute a given bytecodes from a given state.
+@[simp]
+def dispatch (evm: Evm) : Bytecode -> Outcome
+| Bytecode.Stop => STOP evm
+| Bytecode.Add => ADD evm
+| Bytecode.Sub => SUB evm
+| Bytecode.Mul => MUL evm
+| Bytecode.Div => DIV evm
+| Bytecode.Pop => POP evm
+| Bytecode.Dup n => DUP evm n
+| Bytecode.Push n => PUSH evm n
+
+-- Execute a sequence of zero or more bytecodes from a given state.
+@[simp]
+def eval (code: List Bytecode)(evm:Evm) : Outcome :=
+  reduce code (Ok evm)
+where
+   @[simp] reduce : (List Bytecode) -> Outcome -> Outcome
+    | _,(Error err) => Error err
+    | _,(Done gas data) => Done gas data
+    | [], o => o
+    | code::rest,(Ok evm) => reduce rest (dispatch evm code)
+
+/- =============================================================== -/
+/- Tests -/
+/- =============================================================== -/
+
+-- Executing PUSH then POP on an Evm is a no-op.
+example (evm:Evm): (eval [Push n,Pop] evm) = Ok evm :=
+by
+  match evm with
+  | {stack:=h::t} => simp
+  | {stack:=[]} => simp
+
+-- Executing PUSH, PUSH, ADD on an Evm always succeeds.
+example (evm:Evm): ∃evm', (eval [Push n, Push m, Add] evm) = Ok evm' :=
+by
+  simp
+
+-- Executing DUP0 has the right effect
+example (evm:Evm): ∃evm', (eval [Push n, Dup_0] evm) = (Ok evm') :=
+by
+  exists {stack := n::n::evm.stack}
+  simp [*]
+
+-- Executing DUP1 has the right effect
+example (evm:Evm): ∃evm', (eval [Push n, Push m, Dup_1] evm) = (Ok evm') :=
+by
+  exists {stack := n::m::n::evm.stack}
+  simp [*]
+
+-- Executing DUP2 has the right effect
+example (evm:Evm): ∃evm', (eval [Push n, Push m, Push l, Dup_2] evm) = (Ok evm') :=
+by
+  exists {stack := n::l::m::n::evm.stack}
+  simp [*]  
+  simp_arith
