src/LeanEVM/Instructions/Arithmetic.lean
@@ -1,0 +1,142 @@
+import LeanEVM.State
+
+open Exception
+open Outcome
+
+-- ==================================================================
+-- Add
+-- ==================================================================
+
+-- Unsigned integer addition with modulo arithmetic
+@[simp]
+def ADD (evm: Evm) : Outcome :=
+  if r:evm.stack.length > 1
+  then
+    let lhs : u256 := evm.peek 0 (by linarith);
+    let rhs : u256 := evm.peek 1 (by simp [r]);
+    let res : u256 := (u256.add lhs rhs);
+    -- Take operands off stack
+    let evm' := evm.pop 2 r;
+    -- Push result on stack
+    Ok (evm'.push res)
+  else
+    Error StackUnderflow
+
+-- Executing ADD on an empty Evm produces a stack overflow.
+example : (ADD EmptyEvm) = (Error StackUnderflow) :=
+by
+  simp
+
+-- Executing ADD on Evm with two operands succeeds.
+lemma AddOK(rest:List u256): exists evm, (ADD {stack:=l::r::rest}) = (Ok evm) :=
+by
+  exists {stack := (Fin.add l r)::rest}
+  match rest with
+  | h::t => simp; unfold u256.add; rfl
+  | [] => simp; unfold u256.add; rfl
+
+-- ==================================================================
+-- Sub
+-- ==================================================================
+
+-- Unsigned integer subtraction with modulo arithmetic
+@[simp]
+def SUB (evm: Evm) : Outcome :=
+  if r:evm.stack.length > 1
+  then
+    let lhs : u256 := evm.peek 0 (by linarith);
+    let rhs : u256 := evm.peek 1 (by simp [r]);
+    let res : u256 := (u256.sub lhs rhs);
+    -- Take operands off stack
+    let evm' := evm.pop 2 r;
+    -- Push result on stack
+    Ok (evm'.push res)
+  else
+    Error StackUnderflow    
+
+-- Test 0-1 = MAX
+example (rest:List u256): exists evm, (SUB {stack:=U256_0::U256_1::rest}) = (Ok evm) :=
+by
+  exists {stack := U256_MAX::rest}
+  match rest with
+  | h::t => simp; unfold u256.sub; rfl
+  | [] => simp; unfold u256.sub; rfl
+
+-- Test 3-1 = 2
+example (rest:List u256): exists evm, (SUB {stack:=U256_3::U256_2::rest}) = (Ok evm) :=
+by
+  exists {stack := U256_1::rest}
+  match rest with
+  | h::t => simp; unfold u256.sub; rfl
+  | [] => simp; unfold u256.sub; rfl  
+
+-- ==================================================================
+-- Mul
+-- ==================================================================
+
+-- Unsigned integer multiplication with modulo arithmetic
+@[simp]
+def MUL (evm: Evm) : Outcome :=
+  if r:evm.stack.length > 1
+  then
+    let lhs : u256 := evm.peek 0 (by linarith);
+    let rhs : u256 := evm.peek 1 (by simp [r]);
+    let res : u256 := (u256.mul lhs rhs);
+    -- Take operands off stack
+    let evm' := evm.pop 2 r;
+    -- Push result on stack
+    Ok (evm'.push res)
+  else
+    Error StackUnderflow  
+
+-- Test 1*2 = 2
+example (rest:List u256): exists evm, (MUL {stack:=U256_1::U256_2::rest}) = (Ok evm) :=
+by
+  exists {stack := U256_2::rest}
+  match rest with
+  | h::t => simp; unfold u256.mul; rfl
+  | [] => simp; unfold u256.mul; rfl
+
+-- Test 2*2 = 4
+example (rest:List u256): exists evm, (MUL {stack:=U256_2::U256_2::rest}) = (Ok evm) :=
+by
+  exists {stack := U256_4::rest}
+  match rest with
+  | h::t => simp; unfold u256.mul; rfl
+  | [] => simp; unfold u256.mul; rfl
+
+-- ==================================================================
+-- Div
+-- ==================================================================
+
+-- Unsigned integer division with modulo arithmetic
+@[simp]
+def DIV (evm: Evm) : Outcome :=
+  if r:evm.stack.length > 1
+  then
+    let lhs : u256 := evm.peek 0 (by linarith);
+    let rhs : u256 := evm.peek 1 (by simp [r]);
+    let res : u256 := (u256.div lhs rhs);
+    -- Take operands off stack
+    let evm' := evm.pop 2 r;
+    -- Push result on stack
+    Ok (evm'.push res)
+  else
+    Error StackUnderflow  
+
+-- Test 4/2 = 2
+example (rest:List u256): exists evm, (DIV {stack:=U256_4::U256_2::rest}) = (Ok evm) :=
+by
+  exists {stack := U256_2::rest}
+  match rest with
+  | h::t => simp; unfold u256.div; rfl
+  | [] => simp; unfold u256.div; rfl
+
+-- Test 1/0 = 0
+example (rest:List u256): exists evm, (DIV {stack:=U256_1::U256_0::rest}) = (Ok evm) :=
+by
+  exists {stack := U256_0::rest}
+  match rest with
+  | h::t => simp; unfold u256.div; rfl
+  | [] => simp; unfold u256.div; rfl
+
