src/LeanEVM/Instructions/ControlFlow.lean
@@ -1,0 +1,18 @@
+import LeanEVM.State
+
+open Exception
+open Outcome
+
+-- ==================================================================
+-- Stop
+-- ==================================================================
+
+-- Halt the machine without any return data
+@[simp]
+def STOP (_: Evm) : Outcome :=
+  Done 0 Array.empty
+
+-- Executing STOP on an arbitrary Evm produces Done.
+example (evm:Evm) : (STOP evm) = (Done 0 Array.empty) :=
+by
+  rfl
