src/LeanEVM/Instructions/Stack.lean
@@ -1,0 +1,53 @@
+import LeanEVM.State
+
+open Exception
+open Outcome
+
+-- ==================================================================
+-- Push N
+-- ==================================================================
+
+@[simp]
+def PUSH (evm: Evm)(n:u256) : Outcome :=
+  Ok (evm.push n)
+
+-- ==================================================================
+-- Pop
+-- ==================================================================
+
+-- Pop word from stack
+@[simp]
+def POP (evm: Evm) : Outcome :=
+  if r:evm.stack.length > 0
+  then
+    Ok (evm.pop 1 r)
+  else
+    Error StackUnderflow
+
+-- Executing POP on Evm with at least one operand succeeds.
+lemma PopOK (st:List u256)(p:st = v::rest): (POP {stack:=st}) = (Ok {stack:=rest}) :=
+by
+  simp [p]
+  match rest with
+  | h::t => simp
+  | [] => simp
+
+-- Executing PUSH then POP on an Evm is a no-op.
+example (evm:Evm): ((PUSH evm n).apply POP) = Ok evm :=
+by
+  match evm with
+  | {stack:=h::t} => simp
+  | {stack:=[]} => simp
+
+-- ==================================================================
+-- Dup N
+-- ==================================================================
+
+@[simp]
+def DUP (evm: Evm)(n:u4) : Outcome :=
+  if r:evm.stack.length > n.val
+  then
+    let val : u256 := evm.peek n.val (by simp [r]);
+    Ok (evm.push val)
+  else
+    Error StackUnderflow
